chore: Array cleanup (#5782)
More cleanup of Array API. More to come.

src/Std/Sat/AIG/Basic.lean
@@ -128,7 +128,7 @@ theorem Cache.get?_property {decls : Array (Decl α)} {idx : Nat} (c : Cache α 
   induction hcache generalizing decl with
   | empty => simp at hfound
   | push_id wf ih =>
-    rw [Array.get_push]
+    rw [Array.getElem_push]
     split
     · apply ih
       simp [hfound]
@@ -140,7 +140,7 @@ theorem Cache.get?_property {decls : Array (Decl α)} {idx : Nat} (c : Cache α 
       assumption
   | push_cache wf ih =>
     rename_i decl'
-    rw [Array.get_push]
+    rw [Array.getElem_push]
     split
     · simp only [HashMap.getElem?_insert] at hfound
       match heq : decl == decl' with
@@ -464,7 +464,7 @@ def mkGate (aig : AIG α) (input : GateInput aig) : Entrypoint α :=
   let cache := aig.cache.noUpdate
   have invariant := by
     intro i lhs' rhs' linv' rinv' h1 h2
-    simp only [Array.get_push] at h2
+    simp only [Array.getElem_push] at h2
     split at h2
     · apply aig.invariant <;> assumption
     · injections
@@ -483,7 +483,7 @@ def mkAtom (aig : AIG α) (n : α) : Entrypoint α :=
   let cache := aig.cache.noUpdate
   have invariant := by
     intro i lhs rhs linv rinv h1 h2
-    simp only [Array.get_push] at h2
+    simp only [Array.getElem_push] at h2
     split at h2
     · apply aig.invariant <;> assumption
     · contradiction
@@ -499,7 +499,7 @@ def mkConst (aig : AIG α) (val : Bool) : Entrypoint α :=
   let cache := aig.cache.noUpdate
   have invariant := by
     intro i lhs rhs linv rinv h1 h2
-    simp only [Array.get_push] at h2
+    simp only [Array.getElem_push] at h2
     split at h2
     · apply aig.invariant <;> assumption
     · contradiction
