src/Std/Sat/AIG/Lemmas.lean
@@ -78,7 +78,7 @@ The AIG produced by `AIG.mkGate` agrees with the input AIG on all indices that a
 theorem mkGate_decl_eq idx (aig : AIG α) (input : GateInput aig) {h : idx < aig.decls.size} :
     have := mkGate_le_size aig input
     (aig.mkGate input).aig.decls[idx]'(by omega) = aig.decls[idx] := by
-  simp only [mkGate, Array.get_push]
+  simp only [mkGate, Array.getElem_push]
   split
   · rfl
   · contradiction
@@ -99,13 +99,13 @@ theorem denote_mkGate {aig : AIG α} {input : GateInput aig} :
     unfold denote denote.go
   split
   · next heq =>
-    rw [mkGate, Array.get_push_eq] at heq
+    rw [mkGate, Array.getElem_push_eq] at heq
     contradiction
   · next heq =>
-    rw [mkGate, Array.get_push_eq] at heq
+    rw [mkGate, Array.getElem_push_eq] at heq
     contradiction
   · next heq =>
-    rw [mkGate, Array.get_push_eq] at heq
+    rw [mkGate, Array.getElem_push_eq] at heq
     injection heq with heq1 heq2 heq3 heq4
     dsimp only
     congr 2
@@ -132,7 +132,7 @@ The AIG produced by `AIG.mkAtom` agrees with the input AIG on all indices that a
 -/
 theorem mkAtom_decl_eq (aig : AIG α) (var : α) (idx : Nat) {h : idx < aig.decls.size} {hbound} :
     (aig.mkAtom var).aig.decls[idx]'hbound = aig.decls[idx] := by
-  simp only [mkAtom, Array.get_push]
+  simp only [mkAtom, Array.getElem_push]
   split
   · rfl
   · contradiction
@@ -149,14 +149,14 @@ theorem denote_mkAtom {aig : AIG α} :
   unfold denote denote.go
   split
   · next heq =>
-    rw [mkAtom, Array.get_push_eq] at heq
+    rw [mkAtom, Array.getElem_push_eq] at heq
     contradiction
   · next heq =>
-    rw [mkAtom, Array.get_push_eq] at heq
+    rw [mkAtom, Array.getElem_push_eq] at heq
     injection heq with heq
     rw [heq]
   · next heq =>
-    rw [mkAtom, Array.get_push_eq] at heq
+    rw [mkAtom, Array.getElem_push_eq] at heq
     contradiction
 
 /--
@@ -172,7 +172,7 @@ The AIG produced by `AIG.mkConst` agrees with the input AIG on all indices that 
 theorem mkConst_decl_eq (aig : AIG α) (val : Bool) (idx : Nat) {h : idx < aig.decls.size} :
     have := mkConst_le_size aig val
     (aig.mkConst val).aig.decls[idx]'(by omega) = aig.decls[idx] := by
-  simp only [mkConst, Array.get_push]
+  simp only [mkConst, Array.getElem_push]
   split
   · rfl
   · contradiction
@@ -188,14 +188,14 @@ theorem denote_mkConst {aig : AIG α} : ⟦(aig.mkConst val), assign⟧ = val :=
   unfold denote denote.go
   split
   · next heq =>
-    rw [mkConst, Array.get_push_eq] at heq
+    rw [mkConst, Array.getElem_push_eq] at heq
     injection heq with heq
     rw [heq]
   · next heq =>
-    rw [mkConst, Array.get_push_eq] at heq
+    rw [mkConst, Array.getElem_push_eq] at heq
     contradiction
   · next heq =>
-    rw [mkConst, Array.get_push_eq] at heq
+    rw [mkConst, Array.getElem_push_eq] at heq
     contradiction
 
 /--
